\documentclass[12pt]{article}
\usepackage{bigints}
\usepackage{graphicx}			% Use this package to include images
\usepackage{amsmath}	
\usepackage{amssymb}
\usepackage{amsfonts}
\usepackage{polynom}
\usepackage{listings}
% A library of many standard math expressions
\graphicspath{ {./Images/} }
\usepackage[margin=1in]{geometry}% Sets 1in margins. 
\newcommand{\qed}[0]{$\blacksquare$}
\usepackage{fancyhdr}			% Creates headers and footers
\usepackage{enumerate}          %These two package give custom labels to a list
\usepackage[shortlabels]{enumitem}


% Creates the header and footer. You can adjust the look and feel of these here.
\pagestyle{fancy}
\fancyhead[l]{Aditya Gupta}
\fancyhead[c]{Math 136 Homework \#5}
\fancyhead[r]{\today}
\fancyfoot[c]{\thepage}
\renewcommand{\headrulewidth}{0.2pt} %Creates a horizontal line underneath the header
\setlength{\headheight}{15pt} %Sets enough space for the header
\begin{document}
\begin{enumerate}
\item \begin{enumerate}
    \item The projection onto \( \text{Ran } A \) is given by 
    \[
    P_{\text{Ran } A} = A(A^*A)^{-1}A^*
    \]
    This projects any vector in \( \mathbb{C}^m \) onto the column space of \( A \), assuming \( A^*A \) is invertible.

    \item The projection onto \( \text{Ker } A^* \) is 
    \[
    P_{\text{Ker } A^*} = I - A(A^*A)^{-1}A^*
    \]
    Since \( \mathbb{C}^m = \text{Ran } A \oplus \text{Ker } A^* \), this projects orthogonally onto the null space of \( A^* \).

    \item The projection onto \( \text{Ran } A^* \) is 
    \[
    P_{\text{Ran } A^*} = A^*(AA^*)^{-1}A
    \]
    This projects vectors in \( \mathbb{C}^n \) onto the row space of \( A \), which is the column space of \( A^* \).

    \item The projection onto \( \text{Ker } A \) is 
    \[
    P_{\text{Ker } A} = I - A^*(AA^*)^{-1}A
    \]
    Since \( \mathbb{C}^n = \text{Ran } A^* \oplus \text{Ker } A \), this expression projects orthogonally onto the null space of \( A \).
\end{enumerate}

\item 
Let \( L: V \to V \) be a linear transformation on an inner product space \( V \) that is self-adjoint, i.e., it satisfies
\[
\langle u, L(v) \rangle = \langle L(u), v \rangle \quad \text{for all } u, v \in V.
\]

Let \( v_\lambda \) and \( v_\mu \) be eigenvectors corresponding to distinct eigenvalues \( \lambda \) and \( \mu \) of \( L \), i.e.,
\[
L(v_\lambda) = \lambda v_\lambda, \quad L(v_\mu) = \mu v_\mu, \quad \text{with } \lambda \ne \mu.
\]

By the self-adjoint property, we have:
\[
\langle v_\lambda, L(v_\mu) \rangle = \langle L(v_\lambda), v_\mu \rangle.
\]

Substituting the eigenvalue equations:
\[
\langle v_\lambda, \mu v_\mu \rangle = \langle \lambda v_\lambda, v_\mu \rangle.
\]

Using linearity of the inner product:
\[
\mu \langle v_\lambda, v_\mu \rangle = \lambda \langle v_\lambda, v_\mu \rangle.
\]

Subtracting one side from the other:
\[
(\mu - \lambda) \langle v_\lambda, v_\mu \rangle = 0.
\]

Since \( \mu \ne \lambda \), it follows that:
\[
\langle v_\lambda, v_\mu \rangle = 0.
\]

Thus, \( v_\lambda \perp v_\mu \).

\item 
\begin{enumerate}

\item Apply the Gram-Schmidt process to the set $\{1, x, x^2, x^3\}$ with the inner product 
\[
\langle f, g \rangle = \int_{-1}^{1} f(x)g(x)\, dx.
\]
Let:
\[
f_0 = 1, \quad f_1 = x, \quad f_2 = x^2, \quad f_3 = x^3.
\]
Start with:
\[
p_0(x) = f_0(x) = 1.
\]
Next,
\[
p_1(x) = f_1(x) - \frac{\langle f_1, p_0 \rangle}{\langle p_0, p_0 \rangle} p_0(x)
= x - \frac{0}{2} \cdot 1 = x.
\]
Then,
\[
\langle f_2, p_0 \rangle = \int_{-1}^{1} x^2 \cdot 1\, dx = \frac{2}{3}, \quad \langle p_0, p_0 \rangle = 2,
\]
\[
\langle f_2, p_1 \rangle = \int_{-1}^{1} x^3\, dx = 0.
\]
So,
\[
p_2(x) = x^2 - \frac{1}{3}.
\]
Now compute:
\[
\langle f_3, p_0 \rangle = \int_{-1}^{1} x^3 \cdot 1\, dx = 0, \quad
\langle f_3, p_1 \rangle = \int_{-1}^{1} x^4\, dx = \frac{2}{5}, \quad
\langle p_1, p_1 \rangle = \int_{-1}^{1} x^2\, dx = \frac{2}{3},
\]
\[
\frac{\langle f_3, p_1 \rangle}{\langle p_1, p_1 \rangle} = \frac{2/5}{2/3} = \frac{3}{5}.
\]
Also,
\[
\langle f_3, p_2 \rangle = \int_{-1}^{1} x^3 \left(x^2 - \frac{1}{3}\right)\, dx = 0.
\]
So,
\[
p_3(x) = x^3 - \frac{3}{5}x.
\]

\item Verify that each $p_k(x)$ is a solution of the differential equation:
\[
(1 - x^2)y'' - 2x y' + \lambda y = 0 \quad \text{with } \lambda = k(k+1).
\]

For \( p_0(x) = 1 \):
\[
y = 1, \quad y' = 0, \quad y'' = 0,
\]
\[
\text{LHS} = 0 - 0 + \lambda \cdot 1 = \lambda \Rightarrow \lambda = 0 \Rightarrow k = 0.
\]

For \( p_1(x) = x \):
\[
y = x, \quad y' = 1, \quad y'' = 0,
\]
\[
\text{LHS} = 0 - 2x + \lambda x = x(\lambda - 2) \Rightarrow \lambda = 2 \Rightarrow k = 1.
\]

For \( p_2(x) = x^2 - \frac{1}{3} \):
\[
y' = 2x, \quad y'' = 2,
\]
\[
\text{LHS} = (1 - x^2)(2) - 2x(2x) + \lambda(x^2 - \tfrac{1}{3}) 
= 2(1 - x^2) - 4x^2 + \lambda x^2 - \tfrac{\lambda}{3},
\]
\[
= 2 - 6x^2 + \lambda x^2 - \tfrac{\lambda}{3} = 0.
\]
Matching coefficients:
\[
-6x^2 + \lambda x^2 = 0 \Rightarrow \lambda = 6 \Rightarrow k = 2,
\]
\[
2 - \tfrac{\lambda}{3} = 0 \Rightarrow \lambda = 6.
\]

For \( p_3(x) = x^3 - \frac{3}{5}x \):
\[
y' = 3x^2 - \frac{3}{5}, \quad y'' = 6x,
\]
\[
\text{LHS} = (1 - x^2)(6x) - 2x(3x^2 - \tfrac{3}{5}) + \lambda(x^3 - \tfrac{3}{5}x),
\]
\[
= 6x - 6x^3 - 6x^3 + \tfrac{6}{5}x + \lambda x^3 - \tfrac{3\lambda}{5}x,
\]
\[
= -12x^3 + \tfrac{36}{5}x + \lambda x^3 - \tfrac{3\lambda}{5}x = 0.
\]
Equating coefficients:
\[
-12x^3 + \lambda x^3 = 0 \Rightarrow \lambda = 12 \Rightarrow k = 3,
\]
\[
\tfrac{36}{5}x - \tfrac{3\lambda}{5}x = 0 \Rightarrow \lambda = 12.
\]

\end{enumerate}

\item 
We are given the points: $(1,2,-3),\ (4,2,7),\ (3,1,0),\ (6,-2,2),\ (0,4,-2)$

We want to find the best fit plane of the form: $z = ax + by + c$

Let
\[
A = \begin{bmatrix}
1 & 2 & 1 \\
4 & 2 & 1 \\
3 & 1 & 1 \\
6 & -2 & 1 \\
0 & 4 & 1
\end{bmatrix}, \quad
B = \begin{bmatrix}
-3 \\
7 \\
0 \\
2 \\
-2
\end{bmatrix}
\]

We use the least squares formula:
\[
\begin{bmatrix}
a \\
b \\
c
\end{bmatrix}
= (A^T A)^{-1} A^T B
\]

\[
A^T A = \begin{bmatrix}
62 & 7 & 14 \\
7 & 29 & 7 \\
14 & 7 & 5
\end{bmatrix}, \quad
A^T B = \begin{bmatrix}
37 \\
-4 \\
4
\end{bmatrix}
\]

Solving gives:
\[
\begin{bmatrix}
a \\
b \\
c
\end{bmatrix}
\approx
\begin{bmatrix}
1.2 \\
2.0 \\
-9.2
\end{bmatrix}
\]

Thus, the best fit plane is: $z = 1.2x + 2.0y - 9.2$


\end{enumerate}
\end{document}
